PoS/Invariants.v
@@ -3,9 +3,24 @@ Require Import ssreflect ssrbool ssrnat eqtype ssrfun seq.
 From mathcomp
 Require Import path.
 Require Import Eqdep pred prelude idynamic ordtype pcm finmap unionmap heap coding. 
+Require Import Blockchain Protocol Semantics.
 Set Implicit Arguments.
 Unset Strict Implicit.
 Unset Printing Implicit Defensive.
 
-
 (* Invariants of the execution regarding the blockchain *)
+Definition holds (n : nid) (w : World) (cond : State -> Prop) :=
+  exists (st : State),
+    find n (localState w) = Some st -> cond st.
+
+Definition has_chain (bc : Blockchain) (st : State) : Prop :=
+  btChain (blockTree st) == bc.
+
+Definition chain_sync_agreement (w w' : World) :
+  forall (n n' : nid) (bc bc' : Blockchain),
+    holds n w (has_chain bc) ->
+    reachable w w' ->
+    holds n' w' (has_chain bc') ->
+    size bc' == size bc ->
+    bc == bc'.
+Admitted.
