PoS/Semantics.v
@@ -3,6 +3,7 @@ Require Import ssreflect ssrbool ssrnat eqtype ssrfun seq.
 From mathcomp
 Require Import path.
 Require Import Eqdep pred prelude idynamic ordtype pcm finmap unionmap heap coding. 
+Require Import Relations.
 Require Import Protocol Blockchain.
 Set Implicit Arguments.
 Unset Strict Implicit.
@@ -18,20 +19,31 @@ Record World :=
   mkW {
     localState : StateMap;
     inFlightMsgs : PacketSoup;
+    trace : seq Event;
     }.
+
+Parameter initState : StateMap.
+Definition initWorld := mkW initState [::] [::].
 
 Inductive reliable_step (w w' : World) : Prop :=
 | Idle of w = w'
 
-| Deliver (p : Packet) (st st' : State) (ms : ToSend) of
+| Deliver (p : Packet) (st st' : State) (ms : ToSend) (evs : seq Event) of
       p \in inFlightMsgs w &
+      p != NullPacket &
       find (dst p) (localState w) = Some st &
-      procMsg st (msg p) = (st', ms) &
+      procMsg st (msg p) = (st', ms, evs) &
       w' = mkW (upd (dst p) st' (localState w))
                (ms ++ seq.rem p (inFlightMsgs w))
+               (trace w ++ evs)
 
 | Intern (proc : nid) (t : InternalTransition) (st st' : State) (ms : ToSend) of
       find proc (localState w) = Some st &
       procInt st t = (st', ms) &
       w' = mkW (upd proc st' (localState w))
-               (ms ++ (inFlightMsgs w)).
+               (ms ++ (inFlightMsgs w))
+               [::].
+
+Definition reliable_step_star := clos_refl_trans_n1 _ reliable_step.
+
+Definition reachable (w w' : World) := reliable_step_star w w'.
